

## 3.4 实现定理
实现定理大多数证明采用矢列构造证明，也有采用典范模型的非构造性证明，本文在公理系统中证明。出发点是尝试将 justification logic 还原到模态逻辑上。在证明过程中将看到$\text{application}$是如何和$MP$规则互动的，能看到内化定理对于找到清晰的证明结构的作用，也能看到自动证明的困难是如何使限制实现定理不能诱导出一个实现算法的，也就是为可证的找到清晰的证明结构的实现算法事实上就是自动证明的困难问题。但是退而求其次，可以证明如果已经有公式可证的证明，那么存在一个算法来得到具体的证明结构。这似乎引导人在下水前学会游泳，在没有给出证明前先给出可证性。或者说这暗示着所有的问题都是可证性问题，具体的证明交给一个算法来实现就够了。从信息量上来看，可证性证明的复杂度的确比证明的复杂度要低，实现具体证明中复杂度的提升主要来自内化定理。

<!-- 这个猜测的范围是哪里 -->

### Sign and Language on $\Omega$
$x,x_1,x_2,\cdots$: variable<br>
$\mathbf{Var}$: set of variable<br>
$t,t_1,t_2,\cdots$: term<br>
$\mathbf{Term}$: each variable in $\mathbf{Var}$ is a term. Term is closed under the operators $\cdot,+$ and have the following properties
$$\begin{align*}
    & t\cdot t = t\\
    & t+ t = t\\
    & t_1+t_2 = t_2+t_1\\
\end{align*}$$

For each term $t$ in $\mathbf{Term}$, there is a corresponding unary modal operator $\Box_t$. The formula is recursively defined as following
$$\begin{align*}
    F ::= P\ |\ \neg F\ |\ F\rightarrow F\ |\ \Box_t F
\end{align*}$$

$c,c_1,c_2,\cdots$: constant<br>
$\mathbf{Cons}$: set of constant<br>
A Kripk modal is $\mathcal{M} = (\mathcal{G}, \{\mathcal{R_c}\}_{c\in \mathbf{Cons}}, \mathcal{V})$.

$\nu,\mu$: $\mathcal{M-}assignment$, a function from $\mathbf{Var}$ to $\mathbf{Cons}$ of modal $\mathcal{M}$. 

The satisfy relation recursively defined as following
$$\begin{align*}
    & \mathcal{M}, \omega, \nu \models P \Leftrightarrow P\in \mathcal{V}(P)\\
    & \mathcal{M}, \omega, \nu \models \neg F \Leftrightarrow \mathcal{M}, \omega, \nu \not\models F\\
    & \mathcal{M}, \omega, \nu \models F\rightarrow G \Leftrightarrow \mathcal{M}, \omega, \nu \not\models F \vee \mathcal{M}, \omega, \nu \models G\\
    & \mathcal{M}, \omega, \nu \models \Box_t F \Leftrightarrow \mathcal{M}, \omega, \nu \models \Box_{\nu(t)}F\\
    &\qquad\qquad \Leftrightarrow \forall\omega'\in\mathcal{G},\text{if }\omega\mathcal{R}_{\nu(t)}\omega'\text{ then }\mathcal{M}, \omega', \nu \models F
\end{align*}$$

**Axiom.** for any term $t_1,t_2$
$$\begin{align*}
    &\text{TAUT}\\
    &\text{(identity)} & \Box_{t_1}F\rightarrow \Box_{t_2}F\\
    &(\text{application}) & \Box_{t_1}(F\rightarrow M)\rightarrow(\Box_{t_2} F\rightarrow\Box_{t_1\cdot t_2}M)\\
    &(\text{weaking}) & \Box_{t_1} F\rightarrow\Box_{t_1+t_2} F
\end{align*}$$

The formula schema $\Box_{t_1}F\leftrightarrow\Box_{t_2}F$ defined the frame which have the same accessibility relation. Axiom $\text{application}$ is the generalization of $K$ Axiom , Let $t_1=t_2=t$ and $t\cdot t = t$, we have $\Box_t(F\rightarrow M)\rightarrow(\Box_t F\rightarrow\Box_t M)$. Since the $\text{identity}$ Axiom, the $\text{application}$ Axiom is soundness. Axiom $\text{weaking}$ is a special case of $TAUT: \Box_{t_1}F\rightarrow(\Box_{t_1}F\lor\Box_{t_2}F)$, $\Box_{t_1+t_2}$ is a new accessibility relation extened from $\Box_{t_1}$ and $\Box_{t_2}$ such that $\Box_{t_1+t_2}F$ defined by $\Box_{t_1}F\lor\Box_{t_2}F$.

**Rule.** $(1)MP$, $(2)TNEC$, for each term $t$, inferring $\Box_t F$ from $F$.

<!-- 公理系统定义了可以MP合并，可以吸取扩展的正规框架类 -->

justification logic 只能有一个通达关系，证据不能单独成为关系，证据只能依附在点上存在。如果证据成为单独的关系，$\text{application}$公理将不可靠，会受到赋值的印象，无法定义框架。所以只能用$\text{identity}$公理定义关系全同的框架，从而让一般化的$\text{applicaiton}$公理可靠。$\text{identity}$公理让这个逻辑退化为基本的命题模态逻辑，也正因此，$K$中的公式才能被实现为$\Omega$中的公式。

而$\Omega$这个语言中的公式可以一般的定义通达关系之间的关系，这相当于多模态算子的一个具体工具。完全可以有更多的结构来定义通达关系之间的关系。去除$\text{identity}$公理，我们考虑更多公理的例子<br>
**Example.** $\Box_{x_{i+1}}F\rightarrow\Box_{x_i}F$ 定义了一个逐渐加强的关系序列，例如<了解，知道，理解，掌握>，能够刻画关系强度。<br>
**Example.** 设$x,y,z$为三组不同的变元，公式$\Box_xF\land\Box_yF\rightarrow\Box_zF$定义了关系之间的运算，例如，相信并且有证据就是知道。<br>
**Example.** 有些公式因为使用了函数引入了新的通达关系，意味着模型中将到达新的点，这样的公式不能定义框架类，只能定义模型类。$\Box_{t_i}F\land\Box_{t_j}M\rightarrow\Box_{t_i\times t_j}(F\land M)$ 更强的合并，将证据连在一起。
**Example.** 使用公理$\Box_{t_i}F\leftrightarrow\Diamond_{t_i}F$ and $\Box_{t_i}\Box_{t_j}F\rightarrow\Box_{t_j\circ t_i}F$能够定义一个范畴框架。

**Substitution.** Suppose a substitution on proposition letter in normal modal logic $K$ is 

$\sigma(P_1,P_2,\cdots,P_n) = (F_1,F_2,\cdots,F_n)$,

我们将这个替换在$\Omega$上实现。将一个公式或一个公式序列中出现的$\Box$依次实现为$\Box_t$，设$F_i$中出现了$m$个$\Box$，记$F_i(t_1,t_2,\cdots,t_m)$为将$F_i$中的$m$个$\Box$依次实现为$\Box_{t_1},\Box_{t_2},\cdots,\Box_{t_m}$所得到的公式。同样的，设$(F_1,F_2,\cdots,F_n)$中共出现了$s$个$\Box$，记$(F_1,F_2,\cdots,F_n)(t_1,t_2,\cdots,t_s)$为将$(F_1,F_2,\cdots,F_n)$中的$s$个$\Box$依次实现为$\Box_{t_1},\Box_{t_2},\cdots,\Box_{t_s}$所得到的公式。由$\sigma$在$\Omega$上实现的替换为

$\sigma'(P_1,P_2,\cdots,P_n) = (F_1,F_2,\cdots,F_n)(t_1,t_2,\cdots,t_s)$

**Defination.** A forget function $(\cdot)^\circ:\Omega\to K$ defined by replacing all $\Box_t$ to $\Box$ for any term $t$

### From modal $K$ to $\Omega$
**Theorem.** 如果公式$F$是$K$中的命题重言式，那么存在$\Omega$中的替换$\sigma'$使得$F\sigma'$可证并且$(F\sigma')^\circ = F$

**Proof.** Let $F_1,F_2,\cdots,F_n$ be a proof of $F$ in $K$, we try to prove for each $k\le n$ there is a substitution $\sigma'_k$ in $\Omega$ such that $F_k\sigma'_k$ is provable and $(F_k\sigma'_k)^\circ = F_k$. We proof by induction on $k$, suppose that for all $m\le k$, there is a substitution $\sigma'_m$ in $\Omega$ such that $F_m\sigma'_m$ is provable and $(F_m\sigma'_m)^\circ = F_m$.<br>
**Axiom Case** Suppose that $F_k$ is an instance of axiom $A$ in $\mathbf{PL}$, then there is a substitution $\sigma$ in $K$ such that $A\sigma = F_k$, then $\sigma'$ is a substitution such that $A\sigma'$ also is an instance of axiom $A$ and $(A\sigma')^\circ = F_k$<br>
**Modus Ponens Case** Suppose that $F_k$ is obtained from $F_{m}$ and $F_{n} = F_m\rightarrow F_k$ by modus ponens. Then by induction hypothesis there are substitution $\sigma'_m,\sigma'_n$ such that $F_m\sigma'_m,F_n\sigma'_n$ are provable and $(F_m\sigma'_m)^\circ = F_m,(F_n\sigma'_n)^\circ = F_n$. A new substitution $\sigma_k'$ could be obtained by $\sigma_n'$ limitted on $F_k$ such that $(F_k\sigma_k')^\circ = F_k$, we need to prove taht $F_k\sigma_k'$ is provable. Suppose that $F_n\sigma_n' = M\rightarrow F_k\sigma_k'$. For the purpose of using $MP$, we consider how to make sure the formule $M$ is equal to $F_m\sigma_m'$. Since $M^\circ = (F_m\sigma_m')^\circ = F_m$, the modal operators in the two formulas are completely one-to-one corresponding. Let the terms of each corresponding modal operator be equal, which does not cause any contradictions in the $\mathbf{Var}$. Thus we can safety let $M = F_m\sigma_m'$ such that $F_k\sigma_k'$ is provable by $MP$.  

如果没有建立方程的情况下，赋值是任意的，并不能使用$MP$，例如前提分别为$\Box_{x_1}F\rightarrow\Box_{x_1}F,\Box_{x_1}F\rightarrow\Box_{x_2}F$，遗忘后相同，但是变元约束不同。在任意赋值下是不同的，只有令对应的项相同得到一组变元方程，才能使方程约束下的赋值中可以使用$MP$。这并不是说证明依赖于赋值，而是应该看作一些变元符号变少了。造成这个问题的原因在于证明中并没有考虑后面的步骤，只能先用尽量多的变元，然后再在需要时建立等式，并没有让可用的变元减少。另一方面，相等也不会引起混乱，只要每次引入变元时都引入当前证明中没有用过的变元。

**Theorem.** Suppose that modal formula $F$ is provable in $K$, then there is a modal formula $J$ provable in $\Omega$ such that $J^\circ = F$.

**Proof.** Let $F_1,F_2,\cdots,F_n$ be a proof of $F$ in $K$, we try to prove for each $k\le n$ there is a modal formula $J_k$ provable in $\Omega$ such that $J_k^\circ = F_k$.

we proof by induction on $k$. For $k=1$, $F_k$ is an instance of axiom in $K$. If $F_k$ is a tautology, then by theorem there is a substitution $\sigma'$ such that $F_k\sigma'$ is a modal formula and is provable in $\Omega$ and $(F_k\sigma')^\circ = F_k$. If $F_k$ is an instance of $K$ axiom, suppose that $F_k = \Box(F\rightarrow M)\rightarrow(\Box F\rightarrow \Box M)$ and that there are $s,l$ number $\Box$ in $F,M$. Let $i,j\ge s,l$ and $i\neq j$ then
$$\begin{align*}
    \Delta =\ &\Box_{x_i}(F(x_1,x_2,\cdots,x_s)\rightarrow M(x_1,x_2,\cdots,x_l))\rightarrow\\
    &\quad\quad (\Box_{x_j} F(x_1,x_2,\cdots,x_s)\rightarrow\Box_{x_i\cdot x_j}M(x_1,x_2,\cdots,x_s))
\end{align*}$$
is an instance of $\text{application}$ axiom and $\Delta^\circ = F_k$

For $k\ge 1$, By induction hypothesis, suppose that for each $m\le k$ there is a modal formula $J_m$ provable in $\Omega$ such that $J_m^\circ = F_m$. <br>
**Case:Modus Ponens** Suppose that $F_k$ is obtained from $F_{m}$ and $F_{n} = F_m\rightarrow F_k$ by modus ponens. Then by induction hypothesis there are modal formula $J_m,J_n$ provable in $\Omega$ such that $J_m^\circ = F_m,J_n^\circ = F_n$. Suppose that $J_n = M\rightarrow J_k$ and let $M = J_m$, thus $J_k$ is provable by $MP$ and $J_k^\circ = F_k$ .<br>
**Case:Necessitation** Suppose that $F_k$ is obtained from $F_{m}$ by necessitation. Then by induction hypothesis there is a modal formula $J_m$ provable in $\Omega$ such that $J_m^\circ = F_m$. Let $x_i$ be a variable term not used in the proof, then $\Box_{x_i}J_m$is a modal formula and is provable by $TNEC$ in $\Omega$ and $(\Box_{x_i}J_m)^\circ = F_k$.

### From modal $\Omega$ to $\mathsf{J}$

**Defination.** A realization function $(\cdot)^r:\Omega\to\mathsf{J}$ defined by replacing $\Box_t F$ to $t:F$ for any term in $\Omega$.

**Defination.** A box function $(\cdot)^\Box:\mathsf{J}\to \Omega$ defined by replacing all $t:F$ to $\Box_t F$ for any justification term $t$. The box function is the reverse of realization function.

**Theorem.** Suppose that modal formula $F$ is provable in $\Omega$, then there is a justification formula $J$ provable in $\mathsf{J}$ such that $J^\Box = F$.


**Proof.** Let $F_1,F_2,\cdots,F_n$ be a proof of $F$ in $\Omega$, we try to prove for each $k\le n$ there is a justification formula $J_k$ provable in $\mathsf{J}$ such that $J_k^\Box = F_k$.

we proof by induction on $k$. For $k=1$, $F_k$ is an instance of axiom in $\Omega$, then $F_k^r$ is also an instance of axiom in $\mathsf{J}$ and $(F_k^r)^\Box = F_k$. For $k\ge 1$, By induction hypothesis, suppose that for each $m\le k$ there is a justification formula $J_m$ provable in $\mathsf{J}$ such that $J_m^\Box = F_m$.

**Case:Modus Ponens** Suppose that $F_k$ is obtained from $F_{m}$ and $F_{n} = F_m\rightarrow F_k$ by modus ponens. Then by induction hypothesis there are justification formulas $J_m,J_n$ provable in $\mathsf{J}$ such that $J_m^\Box = F_m,J_n^\Box = F_n$. Since $F_n^r = (F_m\rightarrow F_k)^r = F_m^r\rightarrow F_k^r$ and $J_m = (J_m^\Box)^r = F_m^r$,$J_n = (J_n^\Box)^r = F_n^r$, thus $J_n = J_m\rightarrow F_k^r$, thus $F_k^r$ is provable by $MP$ in $\mathsf{J}$ and $(F_k^r)^\Box = F_k$.

**Case:Necessitation** Suppose that $F_k$ is obtained from $F_{m}$ by $TNEC$. Then by induction hypothesis there is a justification formula $J_m$ provable in $\mathsf{J}$ such that $J_m^\Box = F_m$. By the internalization theorem, there is a closed justification term $t$ such that $t:J_m$ is provable in $\mathsf{J}$. Since there term $t$ is closed justification, there is no variable term in $t$. Suppose that $F_k = \Box_{x}F_m$, there is no constant in term $x$. Let $x = t$, thus $(t:J_m)^\Box = F_k$.

